Modify context_t datatype to include key bounds
the current definitions are insufficient to prove that the child key
sets are included in the grandparents keys ranges. We modify the type of the
context with the aim of including the grandparent upper and lower key bounds.

src/Insert_tree_stack.thy
@@ -6,9 +6,9 @@ definition subtree_indexes :: "node_t \<Rightarrow> nat set" where
 "subtree_indexes n == (
   case n of (l,_) \<Rightarrow>  { 0 .. (length l)})"
 
-definition wellformed_context_1 :: "node_t * nat \<Rightarrow> bool" where
+definition wellformed_context_1 :: "(left_bound *(node_t * nat) * right_bound) \<Rightarrow> bool" where
 "wellformed_context_1 lcsi = (
-let ((l,cs),i) = lcsi in
+let (_,((l,cs),i),_) = lcsi in
 wellformed_tree (Rmbs False) (Node(l,cs))
 & i : (subtree_indexes (l,cs))
 )"
@@ -19,16 +19,16 @@ definition is_subnode :: "(node_t * nat) \<Rightarrow> (node_t * nat) \<Rightarr
   let ((ks,rs),i) = pi in
   Node n = (rs!i))"
                                         
-fun linked_context :: "(node_t * nat) \<Rightarrow> context_t \<Rightarrow> bool" where
+fun linked_context :: "(left_bound * (node_t * nat) * right_bound) \<Rightarrow> context_t \<Rightarrow> bool" where
 "linked_context ni [] = True" |
-"linked_context ni (pi#pis) = (
-  is_subnode ni pi \<and> linked_context pi pis)"
+"linked_context (lb,ni,rb) ((plb,pi,prb)#pis) = (
+  is_subnode ni pi \<and> linked_context (plb,pi,prb) pis)"
 
 definition wellformed_context :: "context_t \<Rightarrow> bool" where
 "wellformed_context xs == (
 case xs of Nil \<Rightarrow> True
 | _ \<Rightarrow> (
-let ((l,cs),i) = last xs in
+let (_,((l,cs),i),_) = last xs in
 wellformed_tree (Rmbs True) (Node(l,cs))
 & linked_context (hd xs) (tl xs)
 & i : (subtree_indexes (l,cs))
@@ -56,7 +56,7 @@ let (f,stk) = dest_ts ts in
 
 Nil \<Rightarrow> (True) (* Nil - focus is wf *)
 
-| (((l,cs),i)#nis) \<Rightarrow> (
+| ((lb,((l,cs),i),rb)#nis) \<Rightarrow> (
   let kl = (case i=0 of 
   True \<Rightarrow> None
   | False \<Rightarrow> Some(l!(i-1)))
